code/Yazi.LZ77.fsti
@@ -1,98 +1,35 @@
 module Yazi.LZ77
 
-module Adler32 = Spec.Adler32
 module B = LowStar.Buffer
+module CB = LowStar.ConstBuffer
 module CFlags = Yazi.CFlags
-module CRC32 = Spec.CRC32
 module HS = FStar.HyperStack
 module I32 = FStar.Int32
+module S = Spec.LZ77
 module SS = Spec.Stream
 module Seq = FStar.Seq
 module ST = FStar.HyperStack.ST
-module U16 = FStar.UInt16
 module U32 = FStar.UInt32
 module U8 = FStar.UInt8
-module Util = Yazi.Util
 
-include Yazi.LZ77.State
+include Yazi.LZ77.Types
 
-noeq type lz77_context = {
-  w_size: U32.t; (* LZ77 window size (32K by default) *)
-  w_bits: U16.t; (* log2 w_size  (8..16) *)
-  w_mask: U16.t; (* w_size - 1 *)
-
-  (* Sliding window. Input bytes are read into the second half of the window,
-   * and move to the first half later to keep a dictionary of at least wSize
-   * bytes. With this organization, matches are limited to a distance of
-   * wSize-MAX_MATCH bytes, but this ensures that IO is always
-   * performed with a length multiple of the block size. Also, it limits
-   * the window size to 64K.
-   * To do: use the user input buffer as sliding window. *)
-  window: B.buffer U8.t;
-
-  (* Actual size of window: 2 * w_size, except when the user input buffer
-   * is directly used as sliding window. *)
-  window_size: U32.t;
-     
-  (* Link to older string with same hash index. To limit the size of this
-   * array to 64K, this link is maintained only for the last 32K strings.
-   * An index in this array is thus a window index modulo 32K.*)
-  prev: B.buffer U16.t;
-
-  head: B.buffer U16.t; (* Heads of the hash chains or NIL. *)
-
-  h_size: U32.t;        (* number of elements in hash table *)
-  h_bits: U16.t;        (* log2 h_size *)
-  h_mask: U16.t;        (* h_size - 1 *)
-
-  (* Number of bits by which ins_h must be shifted at each input
-   * step. It must be such that after MIN_MATCH steps, the oldest
-   * byte no longer takes part in the hash key, that is:
-   *   shift * MIN_MATCH >=h_bits *)
-  shift: U16.t;
-}
-
-type stream_state = B.lbuffer U32.t 5
-
-val read_buf:
-    ss: stream_state
-  -> uncompressed: Ghost.erased (Seq.seq U8.t)
-  -> next_in: B.pointer (B.buffer U8.t)
-  -> buf: B.buffer U8.t
-  -> size: U32.t
-  -> wrap: I32.t
-  -> ST.Stack (U32.t & Ghost.erased (B.buffer U8.t))
-  (requires fun h -> 
-    let len = if U32.v size > SS.avail_in (B.as_seq h ss) then
-      SS.avail_in (B.as_seq h ss)
-    else
-      U32.v size
-    in
-    len > 0 /\
-    B.live h ss /\ ~(B.g_is_null ss) /\
-    B.live h buf /\ ~(B.g_is_null buf) /\
-    HS.disjoint (B.frameOf ss) (B.frameOf buf) /\
-    B.length buf == U32.v size /\
-    SS.next_in_valid h ss next_in /\
-    SS.adler_valid h ss wrap uncompressed)
-  (ensures fun h0 res h1 ->
-  let (len', read) = res in
-  let next_in0 = B.get h0 next_in 0 in
-  let next_in1 = B.get h1 next_in 0 in
-  let s0 = B.as_seq h0 ss in
-  let s1 = B.as_seq h1 ss in
-  let len = if U32.v size > SS.avail_in s0 then
-    SS.avail_in s0
-  else
-    U32.v size
-  in
-  len == U32.v len' /\
-  B.modifies (B.loc_union
-    (B.loc_buffer ss)
-    (B.loc_union (B.loc_buffer next_in) (B.loc_buffer buf))) h0 h1 /\
-  Seq.equal (B.as_seq h1 read) (B.as_seq h0 (B.gsub next_in0 0ul len')) /\
-  SS.avail_in s0 - len == SS.avail_in s1 /\
-  SS.next_in_valid h1 ss next_in /\
-  SS.adler_valid h1 ss wrap (Seq.append uncompressed (B.as_seq h1 read)) /\
-  SS.avail_out s0 == SS.avail_out s1 /\
-  SS.total_out s0 == SS.total_out s1)
+private unfold let hash_range_pre_cond (ctx: lz77_context) (h_range: U32.t) =
+  let open FStar.Mul in
+  U32.v ctx.w_size < U32.v h_range /\ U32.v h_range <= 2 * U32.v ctx.w_size
+  
+val slide_hash:
+    ctx: lz77_context_p
+  -> h_range: U32.t
+  -> ST.Stack unit
+  (requires fun h ->
+    S.context_valid h ctx /\
+    (let ctx' = B.get h (CB.as_mbuf ctx) 0 in
+    (ctx'.w_size == h_range \/ hash_range_pre_cond ctx' h_range) /\
+    S.hash_chain_valid h ctx h_range false))
+  (ensures fun h0 _ h1 ->
+    let ctx' = B.get h0 (CB.as_mbuf ctx) 0 in
+    B.modifies (
+      (B.loc_buffer ctx'.head) `B.loc_union`
+      (if CFlags.fastest then B.loc_none else B.loc_buffer ctx'.prev)) h0 h1 /\
+    S.hash_chain_valid h1 ctx h_range true)
