code/Yazi.LZ77.Types.fst
@@ -1,0 +1,49 @@
+module Yazi.LZ77.Types
+
+module B = LowStar.Buffer
+module CB = LowStar.ConstBuffer
+module LB = Lib.Buffer
+module ST = FStar.HyperStack.ST
+module U16 = FStar.UInt16
+module U32 = FStar.UInt32
+module U8 = FStar.UInt8
+
+noeq type lz77_context = {
+  w_size: U32.t; (* LZ77 window size (32K by default) *)
+  w_bits: U16.t; (* log2 w_size  (8..16) *)
+  w_mask: U16.t; (* w_size - 1 *)
+
+  (* Sliding window. Input bytes are read into the second half of the window,
+   * and move to the first half later to keep a dictionary of at least wSize
+   * bytes. With this organization, matches are limited to a distance of
+   * wSize-MAX_MATCH bytes, but this ensures that IO is always
+   * performed with a length multiple of the block size. Also, it limits
+   * the window size to 64K.
+   * To do: use the user input buffer as sliding window. *)
+  window: B.buffer U8.t;
+
+  (* Actual size of window: 2 * w_size, except when the user input buffer
+   * is directly used as sliding window. *)
+  window_size: U32.t;
+     
+  (* Link to older string with same hash index. To limit the size of this
+   * array to 64K, this link is maintained only for the last 32K strings.
+   * An index in this array is thus a window index modulo 32K.*)
+  prev: B.buffer U16.t;
+
+  head: B.buffer U16.t; (* Heads of the hash chains or NIL. *)
+
+  h_size: U32.t;        (* number of elements in hash table *)
+  h_bits: U16.t;        (* log2 h_size *)
+  h_mask: U16.t;        (* h_size - 1 *)
+
+  (* Number of bits by which ins_h must be shifted at each input
+   * step. It must be such that after MIN_MATCH steps, the oldest
+   * byte no longer takes part in the hash key, that is:
+   *   shift * MIN_MATCH >=h_bits *)
+  shift: U16.t;
+}
+
+type lz77_context_p = ctx: CB.const_buffer lz77_context {CB.length ctx == 1}
+
+type lz77_state_t = B.lbuffer U32.t 8
