code/Yazi.Stream.Types.fsti
@@ -1,0 +1,6 @@
+module Yazi.Stream.Types
+
+module B = LowStar.Buffer
+module U32 = FStar.UInt32
+
+type stream_state_t = B.lbuffer U32.t 5
